reify/reify_triple.v
@@ -1,0 +1,163 @@
+Require Import floyd.proofauto.
+Require Import reverse_defs.
+Require Import MirrorShard.Expr.
+Require Import sep.
+Require Import wrapExpr.
+Require Import types.
+Require Import reify_derives.
+Require Import MirrorShard.ReifyExpr MirrorShard.ReifySepExpr.
+
+Local Open Scope logic.
+
+Existing Instance NullExtension.Espec.
+
+Record Triple := mkTriple
+{ Tdelta : tycontext;
+  Tprop : list expr;
+  Tlocal : list expr;
+  Tsep : list Sep.sexpr;
+  Tcommand : statement;
+  Tpost : ret_assert
+}.
+
+Section denotation.
+
+Variable functions : functions our_types.
+Variable preds : Sep.predicates our_types.
+Variable uvars : Expr.env our_types.
+
+
+Definition reflect_prop e := force_Opt (exprD functions uvars nil e tvProp) False.
+Definition False' (_ : environ) := False.
+Definition reflect_local (e: expr) :=  (force_Opt (exprD functions uvars nil e (Expr.tvType 17)) False').
+
+Definition s_reflect := Sep.sexprD functions preds uvars nil.
+
+Definition reflect_Tprop l :=
+map reflect_prop l.
+
+Definition reflect_Tlocal l :=
+map reflect_local l.
+
+Definition reflect_Tsep l := 
+map (fun e => `(s_reflect e)) l.
+
+Definition PreD t :=
+PROPx (reflect_Tprop (Tprop t)) 
+      ( LOCALx (reflect_Tlocal (Tlocal t)) 
+               (SEPx (reflect_Tsep (Tsep t)))).
+
+Definition TripleD t :=
+  semax (Tdelta t) (PreD t) (Tcommand t) ((Tpost t)).
+
+End denotation.
+                
+(*shouldn't need these, can probably do this as part of reification*)
+Ltac change_eqs' l :=
+try
+match l with
+| ?H :: ?T => match H with
+                | `(eq ?l) (eval_id ?r) => change H with (functions.lift_eq l r)
+              end; change_eqs' T
+end.
+
+Ltac change_eqs :=
+match goal with 
+[ |- semax _ (PROPx ?P (LOCALx ?Q (SEPx ?R))) _ _] => change_eqs Q
+end.
+
+Ltac is_const := false.
+
+
+Ltac reify_exprs isConst es types funcs uvars vars k :=
+  match es with
+    | tt => k uvars funcs (@nil expr)
+    | nil => idtac "nill"; idtac k; k uvars funcs (@nil expr)
+    | (?e, ?es) =>
+      reify_expr ltac:(isConst) e types funcs uvars vars ltac:(fun uvars funcs e =>
+        reify_exprs ltac:(isConst) es types funcs uvars vars ltac:(fun uvars funcs es =>
+          let res := constr:(e :: es) in
+          k uvars funcs res))
+    | ?e :: ?es => idtac "consc";
+      reify_expr ltac:(isConst) e types funcs uvars vars ltac:(fun uvars funcs e =>
+        idtac "cons"; reify_exprs ltac:(isConst) es types funcs uvars vars ltac:(fun uvars funcs es =>
+  let res := constr:(e :: es) in
+          k uvars funcs res))
+  end.
+
+
+Ltac reify_props types funcs uvars vars k := 
+match goal with 
+[ |- semax _ (PROPx ?P (LOCALx ?Q (SEPx ?R))) _ _] =>
+reify_exprs is_const P types funcs uvars (@nil bool) k
+end. 
+
+Ltac reify_props_change types funcs uvars vars  :=
+match goal with 
+[ |- semax _ (PROPx ?P (LOCALx ?Q (SEPx ?R))) _ _] =>
+reify_props types funcs uvars vars 
+ltac:(fun uvars funcs res =>idtac "replace"; 
+ change P with 
+(reflect_Tprop funcs uvars res))
+end.
+
+Ltac reify_locals' types funcs uvars vars k l :=
+match l with
+| nil => k uvars funcs (@nil expr)
+| (`(eq ?e) (eval_id ?v))::?T => 
+  reify_expr ltac:(is_const) e types funcs uvars vars ltac:(
+    fun uvars' funcs' e_r => reify_expr ltac:(is_const) v types funcs' uvars' vars 
+  ltac:(
+        fun uvars'' funcs'' v_r => 
+          reify_locals' types funcs'' uvars'' vars ltac:(
+            fun uvars''' funcs''' rest_r => 
+              let res := constr:((Func 55%nat (e_r :: v_r :: nil)) :: rest_r) in
+              k uvars''' funcs''' res) T))
+end. 
+      
+Ltac reify_locals types funcs uvars vars k :=
+match goal with
+[ |- semax _ (PROPx ?P (LOCALx ?Q (SEPx ?R))) _ _] =>
+reify_locals' types funcs uvars vars k Q
+end.
+
+Ltac reify_locals_change types funcs uvars vars  :=
+match goal with 
+[ |- semax _ (PROPx ?P (LOCALx ?Q (SEPx ?R))) _ _] =>
+reify_locals types funcs uvars vars 
+ltac:(fun uvars funcs res =>idtac "replace"; 
+ replace Q with 
+(reflect_Tlocal funcs uvars res))
+end.
+
+Lemma triple : forall p contents sh q r,
+exists POSTCONDITION,
+semax Delta
+     (PROP  (p = q)
+      LOCAL  (`(eq p) (eval_id _p); `(eq q) (eval_id r))  SEP  (`(lseg LS sh contents p nullval)))
+     (Ssequence (Sset _w (Ecast (Econst_int (Int.repr 0) tint) (tptr tvoid)))
+        Sskip) POSTCONDITION.
+intros. eexists. pose_env. 
+let uv := get_uenv types in 
+let types := get_types in
+let funcs := get_funcs types in
+let preds := get_predicates types in 
+let uenv := get_uenv types in
+reify_locals_change types functions uenv uenv. 
+ltac:(fun a b c => id_this (a, b, c)).
+
+let uv := get_uenv types in 
+let types := get_types in
+let funcs := get_funcs types in
+let preds := get_predicates types in 
+let uenv := get_uenv types in
+(*reify_expr is_const (p=q) types funcs uvars (@nil bool) ltac:(fun a b c => idtac "called").*)
+reify_props_change types funcs uenv (@nil bool). 
+replace ((p=q) :: nil) with ( Equal (tvType 4) (Func 55%nat nil) (Func 56%nat nil) :: nil).
+
+match goal with 
+[ |- semax _ (PROPx ?P (LOCALx ?Q (SEPx ?R))) _ _] =>
+end.
+
+change (`(eq p) (eval_id _p)) with (lift_eq p _p).
+intros. eexists.
