reify/sumarray_defs.v
@@ -1,0 +1,80 @@
+Require Import floyd.proofauto.
+Require Export progs.sumarray.
+
+Definition add_elem (f: Z -> val) (i: Z) := Int.add (force_int (f i)).
+
+
+Definition Delta := 
+      (PTree.Node
+         (PTree.Node
+            (PTree.Node PTree.Leaf None
+               (PTree.Node PTree.Leaf (Some (tint, true)) PTree.Leaf)) None
+            (PTree.Node
+               (PTree.Node PTree.Leaf (Some (tptr tint, true)) PTree.Leaf)
+               None (PTree.Node PTree.Leaf (Some (tint, false)) PTree.Leaf)))
+         None
+         (PTree.Node
+            (PTree.Node PTree.Leaf None
+               (PTree.Node PTree.Leaf (Some (tint, true)) PTree.Leaf)) None
+            (PTree.Node
+               (PTree.Node PTree.Leaf (Some (tint, true)) PTree.Leaf) None
+               PTree.Leaf)), PTree.empty type, tint,
+      PTree.Node
+        (PTree.Node
+           (PTree.Node
+              (PTree.Node
+                 (PTree.Node PTree.Leaf
+                    (Some (Global_var (Tarray tint 4 noattr))) PTree.Leaf)
+                 (Some
+                    (Global_func
+                       (WITH _ : unit PRE  [(1%positive, tptr tvoid),
+                        (2%positive, tptr tvoid), (3%positive, tuint),
+                        (4%positive, tuint)](fun _ : environ => !!False)
+                        POST  [tvoid](fun _ : environ => !!False))))
+                 PTree.Leaf) None PTree.Leaf) None PTree.Leaf) None
+        (PTree.Node
+           (PTree.Node
+              (PTree.Node
+                 (PTree.Node PTree.Leaf
+                    (Some
+                       (Global_func
+                          (WITH u : unit PRE  []main_pre prog u POST  [tint]
+                           main_post prog u))) PTree.Leaf)
+                 (Some
+                    (Global_func
+                       (WITH _ : unit PRE  [(1%positive, tptr tschar),
+                        (2%positive, tint)](fun _ : environ => !!False) POST 
+                        [tint](fun _ : environ => !!False)))) PTree.Leaf)
+              None PTree.Leaf) None
+           (PTree.Node PTree.Leaf
+              (Some
+                 (Global_func
+                    (WITH _ : unit PRE  [(1%positive, tdouble)]
+                     (fun _ : environ => !!False) POST  [tdouble]
+                     (fun _ : environ => !!False))))
+              (PTree.Node PTree.Leaf
+                 (Some
+                    (Global_func
+                       (WITH  p : val * share * (Z -> val), size0 : Z PRE 
+                        [(_a, tptr tint), (_n, tint)]
+                        (let (p0, contents0) := p in
+                         let (a1, sh0) := p0 in
+                         PROP  (0 <= size0 <= Int.max_signed;
+                         forall i0 : Z,
+                         0 <= i0 < size0 -> is_int (contents0 i0))
+                         LOCAL  (`(eq a1) (eval_id _a);
+                         `(eq (Vint (Int.repr size0))) (eval_id _n);
+                         `isptr (eval_id _a))
+                         SEP 
+                         (`(array_at tint sh0 contents0 0 size0) (eval_id _a)))
+                        POST  [tint]
+                        (let (p0, contents0) := p in
+                         let (a1, sh0) := p0 in
+                         fun x1 : environ =>
+                         local
+                           (`(eq
+                                (Vint
+                                   (fold_range (add_elem contents0) Int.zero
+                                      0 size0))) retval) x1 &&
+                         `(array_at tint sh0 contents0 0 size0 a1) x1))))
+                 PTree.Leaf)))).
