reify/types.v
@@ -67,6 +67,12 @@ Definition bool_type :=
       ; Expr.Eqb := eqb
       ; Expr.Eqb_correct := eqb_prop |}).
 
+Definition val_map_type  :=
+no_eqb_type  (Z -> val).
+
+Definition lift_prop_type :=
+no_eqb_type (environ -> Prop).
+
 (* equality for comparisons; apparently doesn't exist? *)
 Definition eqb_comparison (c1 c2 : comparison) : bool :=
   match (c1, c2) with
@@ -106,8 +112,10 @@ Definition our_types :=(cons tycontext_type
                        (cons positive_type
                        (cons bool_type
                        (cons comparison_type
-                       (cons tc_assert_type nil
-                       )))))))))))))))).
+                       (cons tc_assert_type 
+                       (cons val_map_type 
+                       (cons lift_prop_type nil
+                       )))))))))))))))))).
 
 Definition tycontext_tv := Expr.tvType 0.
 Definition c_expr_tv := Expr.tvType 1.
@@ -125,3 +133,5 @@ Definition positive_tv := Expr.tvType 12.
 Definition bool_tv := Expr.tvType 13.
 Definition comparison_tv := Expr.tvType 14.
 Definition tc_assert_tv := Expr.tvType 15.
+Definition val_map_tv := Expr.tvType 16.
+Definition lift_prop_tv := Expr.tvType 17.
